Translate TLA+ liveness, start proofs about enabled transitions

hpaxos.thy
@@ -452,6 +452,8 @@ fun Process :: "Acceptor \<Rightarrow> PreMessage \<Rightarrow> State \<Rightarr
                     else recent_msgs st x\<rparr>
   )"
 
+(**)
+
 (* Process1a as a predicate *)
 fun Process1a :: "Acceptor \<Rightarrow> PreMessage \<Rightarrow> State \<Rightarrow> State \<Rightarrow> bool" where
   "Process1a a m st st2 = (
@@ -461,7 +463,7 @@ fun Process1a :: "Acceptor \<Rightarrow> PreMessage \<Rightarrow> State \<Righta
     \<and> Store_acc a m st st2
     \<and> (if WellFormed st new1b
        then 
-          Send new1b sSt st2
+          Send new1b st st2
           \<and> (recent_msgs st2 = (
               \<lambda>a2. if a2 = a then [] 
                              else recent_msgs st a2))
