hpaxos_liveness.thy
@@ -1,32 +1,286 @@
 theory hpaxos_liveness
-imports Main hpaxos hpaxos_safety
+imports Main hpaxos
 begin
 
+fun Enabled :: "(State \<Rightarrow> State \<Rightarrow> bool) \<Rightarrow> State \<Rightarrow> bool" where
+  "Enabled r st = (\<exists>st2. r st st2)"
+
+(* Send1a is always enabled.*)
+lemma Send1a_Enabled:
+  shows "Enabled (Send1a b) st = True"
+  by fastforce
+
+lemma Process1aAlt1:
+  assumes "WellFormed st (M1b a (m # recent_msgs st a))"
+      and "type m = T1a"
+      and "Recv_acc st a m"
+    shows "Process1a a m st (st\<lparr>msgs := M1b a (m # recent_msgs st a) # msgs st, 
+                                recent_msgs := (
+                                  \<lambda>a2. if a2 = a then [] 
+                                                 else recent_msgs st a2),
+                                queued_msg := (
+                                  \<lambda>a2. if a2 = a then Some (M1b a (m # recent_msgs st a)) 
+                                                 else queued_msg st a2),
+                                known_msgs_acc := (
+                                  \<lambda>x. if a = x 
+                                      then m # known_msgs_acc st x
+                                      else known_msgs_acc st x) \<rparr>)"
+proof -
+  define st2 where "st2 = (st\<lparr>msgs := M1b a (m # recent_msgs st a) # msgs st, 
+                              recent_msgs := (
+                                \<lambda>a2. if a2 = a then [] 
+                                               else recent_msgs st a2),
+                              queued_msg := (
+                                \<lambda>a2. if a2 = a then Some (M1b a (m # recent_msgs st a)) 
+                                               else queued_msg st a2),
+                              known_msgs_acc := (
+                                \<lambda>x. if a = x 
+                                    then m # known_msgs_acc st x
+                                    else known_msgs_acc st x) \<rparr>)"
+  
+  have "Store_acc a m st st2" 
+    by (simp add: st2_def)
+  have "Send (M1b a (m # recent_msgs st a)) st st2
+          \<and> (recent_msgs st2 = (
+              \<lambda>a2. if a2 = a then [] 
+                             else recent_msgs st a2))
+          \<and> (queued_msg st2 = (
+              \<lambda>a2. if a2 = a then Some (M1b a (m # recent_msgs st a)) 
+                             else queued_msg st a2))"
+    by (simp add: st2_def)
+  show ?thesis
+    unfolding Process1a.simps
+    by (smt (verit, ccfv_SIG) \<open>Send (M1b a (m # recent_msgs st a)) st st2 \<and> recent_msgs st2 = (\<lambda>a2. if a2 = a then [] else recent_msgs st a2) \<and> queued_msg st2 = (\<lambda>a2. if a2 = a then Some (M1b a (m # recent_msgs st a)) else queued_msg st a2)\<close> \<open>Store_acc a m st st2\<close> assms(1) assms(2) assms(3) ext_inject st2_def surjective update_convs(1) update_convs(2) update_convs(4) update_convs(5))
+qed
+
+lemma Process1aAlt2:
+  assumes "\<not> WellFormed st (M1b a (m # recent_msgs st a))"
+      and "type m = T1a"
+      and "Recv_acc st a m"
+    shows "Process1a a m st (st\<lparr>recent_msgs := (
+                              \<lambda>a2. if a2 = a then m # recent_msgs st a2 
+                                             else recent_msgs st a2),
+                            known_msgs_acc := (
+                                \<lambda>x. if a = x 
+                                    then m # known_msgs_acc st x
+                                    else known_msgs_acc st x)\<rparr>)"
+proof -
+  define st2 where "st2 = (st\<lparr>recent_msgs := (
+                              \<lambda>a2. if a2 = a then m # recent_msgs st a2 
+                                             else recent_msgs st a2),
+                            known_msgs_acc := (
+                                \<lambda>x. if a = x 
+                                    then m # known_msgs_acc st x
+                                    else known_msgs_acc st x)\<rparr>)"
+  
+  have "Store_acc a m st st2" 
+    by (simp add: st2_def)
+  have "(recent_msgs st2 = (
+              \<lambda>a2. if a2 = a then m # recent_msgs st a2 
+                             else recent_msgs st a2))
+          \<and> (msgs st = msgs st2)
+          \<and> (queued_msg st = queued_msg st2)"
+    by (simp add: st2_def)
+  show ?thesis
+    unfolding Process1a.simps
+    using assms(1) assms(2) assms(3) by auto
+qed
+
+lemma Process1a_Enabled:
+  shows "Enabled (Process1a a m) st = (type m = T1a \<and> Recv_acc st a m)"
+  by (metis (no_types, lifting) Enabled.simps Process1a.simps Process1aAlt1 Process1aAlt2)
+
+lemma Process1bAlt1:
+  assumes "\<forall> mb b :: Ballot. MaxBal st a b \<and> B m b \<longrightarrow> mb \<le> b"
+      and "type m = T1b"
+      and "Recv_acc st a m"
+    shows "Process1b a m st (st\<lparr>recent_msgs := (
+                                      \<lambda>x. if x = a 
+                                          then m # recent_msgs st x
+                                          else recent_msgs st x ),
+                                known_msgs_acc := (
+                                  \<lambda>x. if a = x 
+                                      then m # known_msgs_acc st x
+                                      else known_msgs_acc st x),
+                                two_a_lrn_loop := (\<lambda>x.
+                                    if x = a
+                                    then True
+                                    else two_a_lrn_loop st x),
+                                 processed_lrns := (\<lambda>x.
+                                      if x = a
+                                      then {}
+                                      else processed_lrns st x),
+                                queued_msg := (\<lambda>x.
+                                      if x = a
+                                      then None
+                                      else queued_msg st x) \<rparr>)"
+proof -
+  define st2 where "st2 = st\<lparr>recent_msgs := (
+                                      \<lambda>x. if x = a 
+                                          then m # recent_msgs st x
+                                          else recent_msgs st x ),
+                            known_msgs_acc := (
+                              \<lambda>x. if a = x 
+                                  then m # known_msgs_acc st x
+                                  else known_msgs_acc st x),
+                            two_a_lrn_loop := (\<lambda>x.
+                                if x = a
+                                then True
+                                else two_a_lrn_loop st x),
+                             processed_lrns := (\<lambda>x.
+                                  if x = a
+                                  then {}
+                                  else processed_lrns st x),
+                            queued_msg := (\<lambda>x.
+                                  if x = a
+                                  then None
+                                  else queued_msg st x) \<rparr>"
+  have "recent_msgs st2 = (
+        \<lambda>x. if x = a 
+            then m # recent_msgs st x
+            else recent_msgs st x )" by (simp add: st2_def)
+  have "queued_msg st2 = (\<lambda>x.
+          if x = a
+          then None
+          else queued_msg st x)" by (simp add: st2_def)
+  have "Store_acc a m st st2" by (simp add: st2_def)
+  have "two_a_lrn_loop st2 = (\<lambda>x.
+          if x = a
+          then True
+          else two_a_lrn_loop st x)
+        \<and> processed_lrns st2 = (\<lambda>x.
+          if x = a
+          then {}
+          else processed_lrns st x)" by (simp add: st2_def)
+  have "(msgs st2 = msgs st)
+    \<and> (decision st2 = decision st)
+    \<and> (BVal st2 = BVal st)" by (simp add: st2_def)
+  show ?thesis
+    unfolding Process1b.simps
+    using \<open>Store_acc a m st st2\<close> \<open>msgs st2 = msgs st \<and> decision st2 = decision st \<and> BVal st2 = BVal st\<close> \<open>queued_msg st2 = (\<lambda>x. if x = a then None else queued_msg st x)\<close> \<open>recent_msgs st2 = (\<lambda>x. if x = a then m # recent_msgs st x else recent_msgs st x)\<close> \<open>two_a_lrn_loop st2 = (\<lambda>x. if x = a then True else two_a_lrn_loop st x) \<and> processed_lrns st2 = (\<lambda>x. if x = a then {} else processed_lrns st x)\<close> assms(1) assms(2) assms(3) st2_def by fastforce
+qed
+
+lemma Process1bAlt2:
+  assumes "\<not> (\<forall> mb b :: Ballot. MaxBal st a b \<and> B m b \<longrightarrow> mb \<le> b)"
+      and "type m = T1b"
+      and "Recv_acc st a m"
+    shows "Process1b a m st (st\<lparr>recent_msgs := (
+                                      \<lambda>x. if x = a 
+                                          then m # recent_msgs st x
+                                          else recent_msgs st x ),
+                                known_msgs_acc := (
+                                  \<lambda>x. if a = x 
+                                      then m # known_msgs_acc st x
+                                      else known_msgs_acc st x),
+                                queued_msg := (\<lambda>x.
+                                      if x = a
+                                      then None
+                                      else queued_msg st x) \<rparr>)"
+proof -
+  define st2 where "st2 = st\<lparr>recent_msgs := (
+                                      \<lambda>x. if x = a 
+                                          then m # recent_msgs st x
+                                          else recent_msgs st x ),
+                            known_msgs_acc := (
+                              \<lambda>x. if a = x 
+                                  then m # known_msgs_acc st x
+                                  else known_msgs_acc st x),
+                            queued_msg := (\<lambda>x.
+                                  if x = a
+                                  then None
+                                  else queued_msg st x) \<rparr>"
+  have "recent_msgs st2 = (
+        \<lambda>x. if x = a 
+            then m # recent_msgs st x
+            else recent_msgs st x )" by (simp add: st2_def)
+  have "queued_msg st2 = (\<lambda>x.
+          if x = a
+          then None
+          else queued_msg st x)" by (simp add: st2_def)
+  have "Store_acc a m st st2" by (simp add: st2_def)
+  have "two_a_lrn_loop st2 = two_a_lrn_loop st
+        \<and> processed_lrns st2 = processed_lrns st" by (simp add: st2_def)
+  have "(msgs st2 = msgs st)
+    \<and> (decision st2 = decision st)
+    \<and> (BVal st2 = BVal st)" by (simp add: st2_def)
+  show ?thesis
+    unfolding Process1b.simps
+    using \<open>Store_acc a m st st2\<close> \<open>msgs st2 = msgs st \<and> decision st2 = decision st \<and> BVal st2 = BVal st\<close> \<open>queued_msg st2 = (\<lambda>x. if x = a then None else queued_msg st x)\<close> \<open>recent_msgs st2 = (\<lambda>x. if x = a then m # recent_msgs st x else recent_msgs st x)\<close> \<open>two_a_lrn_loop st2 = two_a_lrn_loop st \<and> processed_lrns st2 = processed_lrns st\<close> assms(1) assms(2) assms(3) st2_def by blast
+qed
+
+lemma Process1b_Enabled:
+  shows "Enabled (Process1b a m) st = (type m = T1b \<and> Recv_acc st a m)"
+  by (smt (verit, best) Enabled.simps Process1b.simps Process1bAlt1 Process1bAlt2)
+
+lemma Process2aAlt:
+  assumes "type m = T2a"
+      and "Recv_acc st a m"
+    shows "Process2a a m st (st\<lparr>recent_msgs := (
+                                  \<lambda>x. if x = a 
+                                      then m # recent_msgs st x
+                                      else recent_msgs st x ),
+                                known_msgs_acc := (
+                                      \<lambda>x. if a = x 
+                                          then m # known_msgs_acc st x
+                                          else known_msgs_acc st x
+                                  )\<rparr>)"
+proof -
+  define st2 where "st2 = st\<lparr>recent_msgs := (
+                                  \<lambda>x. if x = a 
+                                      then m # recent_msgs st x
+                                      else recent_msgs st x ),
+                              known_msgs_acc := (
+                                    \<lambda>x. if a = x 
+                                        then m # known_msgs_acc st x
+                                        else known_msgs_acc st x
+                                )\<rparr>"
+  have "Store_acc a m st st2
+    \<and> recent_msgs st2 = (
+        \<lambda>x. if x = a 
+            then m # recent_msgs st x
+            else recent_msgs st x )
+    \<and> (msgs st2 = msgs st)
+    \<and> (queued_msg st2 = queued_msg st)
+    \<and> (two_a_lrn_loop st2 = two_a_lrn_loop st)
+    \<and> (processed_lrns st2 = processed_lrns st)
+    \<and> (decision st2 = decision st)
+    \<and> (BVal st2 = BVal st)" by (simp add: st2_def)
+  show ?thesis
+    unfolding Process2a.simps
+    using \<open>Store_acc a m st st2 \<and> recent_msgs st2 = (\<lambda>x. if x = a then m # recent_msgs st x else recent_msgs st x) \<and> msgs st2 = msgs st \<and> queued_msg st2 = queued_msg st \<and> two_a_lrn_loop st2 = two_a_lrn_loop st \<and> processed_lrns st2 = processed_lrns st \<and> decision st2 = decision st \<and> BVal st2 = BVal st\<close> assms(1) assms(2) st2_def by fastforce
+qed
+
+lemma Process2a_Enabled:
+  shows "Enabled (Process2a a m) st = (type m = T2a \<and> Recv_acc st a m)"
+  by (metis (no_types, lifting) Enabled.simps Process2a.simps Process2aAlt)
+
+fun Acceptor_Enabled :: "Acceptor \<Rightarrow> State \<Rightarrow> bool" where
+  "Acceptor_Enabled a st = (
+    (\<exists>m. Recv_acc st a m) \<or> (\<exists>ln :: Learner. ln \<notin> processed_lrns st a)
+  )"
+
+(* Process1bLearnerLoop is always enabled.*)
+lemma Process1bLearnerLoop_Enabled:
+  "Enabled (Process1bLearnerLoop a) st = True"
+  sorry
+
+
 (*
-WF_vars(\E v \in Value : LearnerDecide(L, b, v))
+define new1b where "new1b = M1b a (m # recent_msgs st a)"
 *)
 
-(* Send1a is always enabled.
-fun Send1a_Enabled :: "Ballot \<Rightarrow> State \<Rightarrow> bool" where
-  "Send1a_Enabled b st = True"
-*)
-
-fun Process1a_Enabled :: "Acceptor \<Rightarrow> PreMessage \<Rightarrow> State \<Rightarrow> bool" where
-  "Process1a_Enabled a m st = (
-    type m = T1a \<and>
-    Recv_acc st a m
+fun AcceptorProcessAction_Enabled :: "Acceptor \<Rightarrow> State \<Rightarrow> bool" where
+  "AcceptorProcessAction_Enabled a st = (
+    is_safe a \<and> (
+      (\<not> two_a_lrn_loop st a \<and>
+       ((queued_msg st a \<noteq> None \<and> 
+         Process1b_Enabled a (the (queued_msg st a)) st) \<or> 
+        (queued_msg st a = None \<and> (
+          \<exists>m \<in> set (msgs st). Process1a_Enabled a m st \<or> Process1b_Enabled a m st
+        ))))
+      \<or> (two_a_lrn_loop st a))
   )"
 
-fun Process1b_Enabled :: "Acceptor \<Rightarrow> PreMessage \<Rightarrow> State \<Rightarrow> bool" where
-  "Process1b_Enabled a m st = (
-    type m = T1b
-    \<and> Recv_acc st a m
-  )"
-
-(* Process1bLearnerLoop is always enabled.
-fun Process1bLearnerLoop_Enabled :: "Acceptor \<Rightarrow> State \<Rightarrow> bool" where
-  "Process1bLearnerLoop_Enabled a st = True"
-*)
 
 fun LearnerRecv_Enabled :: "Learner \<Rightarrow> PreMessage \<Rightarrow> State \<Rightarrow> bool" where
   "LearnerRecv_Enabled l m st = (
@@ -41,29 +295,60 @@ fun WF :: "(State \<Rightarrow> bool) \<Rightarrow> (State \<Rightarrow> State \
     \<forall>i. (\<forall>j \<ge> i. p_Enabled (f j)) \<longrightarrow> (\<exists>j \<ge> i. p (f j) (f (j + 1)))
   )"
 
+fun BallotLimit1 :: "(nat \<Rightarrow> State) \<Rightarrow> Ballot \<Rightarrow> nat \<Rightarrow> bool" where
+  "BallotLimit1 f b i = (\<forall>m \<in> set (msgs (f i)). type m = T1a \<longrightarrow> bal m < b)"
+
+fun BallotLimit2 :: "(nat \<Rightarrow> State) \<Rightarrow> Ballot \<Rightarrow> bool" where
+  "BallotLimit2 f b = (\<forall>c :: Ballot. c > b \<longrightarrow> (\<forall>j. \<not> (Send1a c (f j) (f (1 + j)))))"
+
+fun BallotSend :: "(nat \<Rightarrow> State) \<Rightarrow> Ballot \<Rightarrow> bool" where
+  "BallotSend f b = (\<forall>i. \<exists>j \<ge> i. Send1a b (f j) (f (j + 1)))"
+
+fun EventuallyProccess1a :: "(nat \<Rightarrow> State) \<Rightarrow> Ballot \<Rightarrow> Acceptor set \<Rightarrow> bool" where
+  "EventuallyProccess1a f b Q = 
+    (\<forall>m :: PreMessage. B m b \<longrightarrow> (\<forall>a \<in> Q. WF (Process1a_Enabled a m) (Process1a a m) f))"
+
+fun EventuallyProccess1b :: "(nat \<Rightarrow> State) \<Rightarrow> Ballot \<Rightarrow> Acceptor set \<Rightarrow> bool" where
+  "EventuallyProccess1b f b Q = 
+    (\<forall>m :: PreMessage. B m b \<longrightarrow> (\<forall>a \<in> Q. WF (Process1b_Enabled a m) (Process1b a m) f))"
+
+fun EventuallyProcess1bLearnerLoop :: "(nat \<Rightarrow> State) \<Rightarrow> Acceptor set \<Rightarrow> bool" where
+  "EventuallyProcess1bLearnerLoop f Q = 
+    (\<forall>a \<in> Q. \<forall>i. \<exists>j \<ge> i. Process1bLearnerLoop a (f j) (f (j + 1)))"
+
+fun EventuallyLearnerRecv :: "(nat \<Rightarrow> State) \<Rightarrow> Learner \<Rightarrow> Ballot \<Rightarrow> bool" where
+  "EventuallyLearnerRecv f L b = 
+    (\<forall>m :: PreMessage. B m b \<longrightarrow> WF (LearnerRecv_Enabled L m) (LearnerRecv L m) f)"
+
+fun EventuallyLearnerDecide :: "(nat \<Rightarrow> State) \<Rightarrow> Learner \<Rightarrow> Ballot \<Rightarrow> bool" where
+  "EventuallyLearnerDecide f L b = 
+    WF (\<lambda>st. \<exists> v :: Value. LearnerDecide_Enabled L b v st) 
+       (\<lambda>st st2. \<exists> v :: Value. LearnerDecide L b v st st2) f"
+
+fun Liveness_Assumptions :: "(nat \<Rightarrow> State) \<Rightarrow> Learner \<Rightarrow> Ballot \<Rightarrow> Acceptor set \<Rightarrow> nat \<Rightarrow> bool" where
+ "Liveness_Assumptions f L b Q i = (
+     BallotLimit1 f b i \<and>
+     BallotLimit2 f b \<and>
+     BallotSend f b \<and>
+     EventuallyProccess1a f b Q \<and>
+     EventuallyProccess1b f b Q \<and>
+     EventuallyProcess1bLearnerLoop f Q \<and>
+     EventuallyLearnerRecv f L b \<and>
+     EventuallyLearnerDecide f L b
+    )"
 
 fun Liveness :: "(nat \<Rightarrow> State) \<Rightarrow> bool" where
   "Liveness f = (
     \<forall> L :: Learner. \<forall> b :: Ballot. \<forall>Q :: Acceptor set. is_quorum Q \<longrightarrow>
-    (\<forall>a \<in> Q. is_safe a) \<and> (
-    TrustLive L Q \<longrightarrow> (
-    ((\<forall>m :: PreMessage. type m = T1a \<longrightarrow> bal m < b) \<and>
-     (\<forall>c :: Ballot. c > b \<longrightarrow> (\<forall>j. \<not> (Send1a c (f j) (f (1 + j))))) \<and>
-     (WF (\<lambda>x. True) (Send1a b) f) \<and>
-     (\<forall>m :: PreMessage. B m b \<longrightarrow> (\<forall>a \<in> Q. WF (Process1a_Enabled a m) (Process1a a m) f)) \<and>
-     (\<forall>m :: PreMessage. B m b \<longrightarrow> (\<forall>a \<in> Q. WF (Process1b_Enabled a m) (Process1b a m) f)) \<and>
-     (\<forall>a \<in> Q. WF (\<lambda>x. True) (Process1bLearnerLoop a) f) \<and>
-     (\<forall>m :: PreMessage. B m b \<longrightarrow> WF (LearnerRecv_Enabled L m) (LearnerRecv L m) f) \<and>
-     (WF (\<lambda>st. \<exists> v :: Value. LearnerDecide_Enabled L b v st) 
-         (\<lambda>st st2. \<exists> v :: Value. LearnerDecide L b v st st2) f)
-    ) \<longrightarrow> (\<exists>j. \<exists> BB :: Ballot . decision (f j) L BB \<noteq> {})
-  )))"
-
+    (\<forall>a \<in> Q. is_safe a) \<longrightarrow> TrustLive L Q \<longrightarrow> 
+    (\<forall>i. Liveness_Assumptions f L b Q i \<longrightarrow> 
+    (\<exists>j \<ge> i. \<exists> BB :: Ballot . decision (f j) L BB \<noteq> {})
+  ))"
 
 
 theorem LivenessResult :
   assumes "Spec f"
   shows "Liveness f"
-sorry
+  sorry
 
 end
